Introducing generic constraints (#4)
* [constraints][1/X] add generics constraints

Add a set of constraints to classDef. They are here to describe
the class level generics constraints. This diff only adds them
in the definitions. Subsequent diffs will make sure they are
well-formed (w.r.t. the class level generics) and they are
valid (especially around New, and class/method/field type check)

* [constraints][2/X] add generics constraints

Added definition on structural wf : all types in the constraints
must be wf and bounded w.r.t. their class generics

* [constraints][3/X] add generics constraints

Adding a set of constraints to all subtyping judgements, and fallout.
No new rules are added, and one admit had to be added into adequacy.

The next diff will add the new subtyping rules to use these constraints
and the necessary checks (New / Class and Method defs), but won't fix
adequacy. The diff after that will tie the knot and fix everything.

* [constraints][4/X] add generics constraints

- Adding a new subtype rule to use the newly introduced constraint set.
- In `NewTy`, checking that the constraints of the newly instanciated
  class are satisfied
- Update interpretation: it is now parametrized by a set of constraints.
  Like the map to interpret remaining generics, it is used to constraint
  them.
- Adequacy is updated to reflect all that. Most of the work has been
  on the method call case

* [constraints][5/X] add generics constraints

Fixing few typos + doc + reorg bits of the code

* [constraints][5/X] add generics constraints

Adding a simple example of a constraint

* Simplifying a definition

theories/examples.v
@@ -12,9 +12,11 @@ From iris.algebra.lib Require Import gmap_view.
 
 From shack Require Import lang progdef subtype typing eval heap modality interp adequacy.
 
+Definition arraykey := UnionT IntT BoolT.
+
 (* TODO: we don't have void atm so I'm using null ;) *)
 
-(* Definition of class ROBox<+T>:
+(* Definition of class ROBox<+T as arraykey>:
  * class ROBox<+T> {
  *   private T $data;
  *   function get(): T { $ret = $this->data; return $ret; }
@@ -31,6 +33,7 @@ Definition ROBox := {|
   classname := "ROBox";
   superclass := None;
   generics := [Covariant];
+  constraints := [(GenT 0, arraykey)];
   classfields := {["$data" := (Private, GenT 0)]};
   classmethods := {["get" := Get]};
 |}.
@@ -54,6 +57,7 @@ Definition Box := {|
   classname := "Box";
   superclass := None;
   generics := [Invariant];
+  constraints := [];
   classfields := {["$data" := (Public, GenT 0)]};
   classmethods := {["set" := BoxSet; "get" := Get]};
 |}.
@@ -77,6 +81,7 @@ Definition IntBoxS := {|
   classname := "IntBoxS";
   superclass := Some ("Box", σ);
   generics := [];
+  constraints := [];
   classfields := ∅;
   classmethods := {["set" := IntBoxSSet]};
 |}.
@@ -116,6 +121,7 @@ Definition Main := {|
   classname := "Main";
   superclass := None;
   generics := [];
+  constraints := [];
   classfields := ∅;
   classmethods := {["entry_point" := EntryPoint]};
  |}.
@@ -313,7 +319,7 @@ Definition final_lty lty : local_tys :=
   (<["$robox" := ClassT "ROBox" [IntT]]> lty)))).
 
 Lemma Main_ty lty :
-  cmd_has_ty lty ProgramBody (final_lty lty).
+  cmd_has_ty [] lty ProgramBody (final_lty lty).
 Proof.
   rewrite /final_lty /ProgramBody.
   eapply SeqTy.
@@ -321,6 +327,14 @@ Proof.
     + econstructor => //.
       move => k ty; rewrite list_lookup_singleton_Some.
       case => _ <-; by constructor.
+    + econstructor => //.
+      * move => i ty.
+        rewrite list_lookup_singleton_Some => [[? <-]].
+        by constructor.
+      * rewrite /ROBox /= => i [??] h.
+        apply list_lookup_singleton_Some in h as [? heq].
+        case: heq => <- <- /=.
+        by eauto.
     + by apply has_fields_ROBox.
     + by set_solver.
     + move => f fty arg.
@@ -338,6 +352,7 @@ Proof.
   }
   eapply SeqTy.
   { eapply NewTy with (targs := []).
+    + by econstructor.
     + by econstructor.
     + by apply has_fields_IntBoxS.
     + by set_solver.
@@ -406,7 +421,7 @@ Proof.
       by rewrite lookup_insert_ne.
 Qed.
 
-Lemma wf_mdef_ty_Main: wf_mdef_ty "Main" (gen_targs 0) (gen_targs 0) EntryPoint.
+Lemma wf_mdef_ty_Main: wf_mdef_ty [] "Main" (gen_targs 0) EntryPoint.
 Proof.
   rewrite /wf_mdef_ty.
   exists (final_lty {| type_of_this := ("Main", gen_targs 0); ctxt := subst_ty (gen_targs 0) <$> methodargs EntryPoint|}).
@@ -1048,11 +1063,139 @@ Proof.
   done.
 Qed.
 
+Lemma wf_constraints_wf : map_Forall (λ _cname, wf_cdef_constraints_wf) Δ.
+Proof.
+  rewrite map_Forall_lookup => c0 d0.
+  rewrite lookup_insert_Some.
+  case => [[? <-]|[?]].
+  { rewrite /wf_cdef_constraints_wf /ROBox /= Forall_singleton.
+    split; by constructor.
+  }
+  rewrite lookup_insert_Some.
+  case => [[? <-]|[?]].
+  { by rewrite /wf_cdef_constraints_wf /= Forall_nil. }
+  rewrite lookup_insert_Some.
+  case => [[? <-]|[?]].
+  { by rewrite /wf_cdef_constraints_wf /= Forall_nil. }
+  rewrite lookup_singleton_Some.
+  case => [? <-].
+  by rewrite /wf_cdef_constraints_wf /= Forall_nil.
+Qed.
+
+  
+Lemma wf_constraints_bounded : map_Forall (λ _cname, wf_cdef_constraints_bounded) Δ.
+Proof.
+  rewrite map_Forall_lookup => c0 d0.
+  rewrite lookup_insert_Some.
+  case => [[? <-]|[?]].
+  { rewrite /wf_cdef_constraints_bounded /= Forall_singleton.
+    split; by repeat constructor.
+  }
+  rewrite lookup_insert_Some.
+  case => [[? <-]|[?]].
+  { by rewrite /wf_cdef_constraints_bounded /= Forall_nil. }
+  rewrite lookup_insert_Some.
+  case => [[? <-]|[?]].
+  { by rewrite /wf_cdef_constraints_bounded /= Forall_nil. }
+  rewrite lookup_singleton_Some.
+  case => [? <-].
+  by rewrite /wf_cdef_constraints_bounded /= Forall_nil.
+Qed.
+
+Lemma wf_parent_ok : map_Forall (λ _cname, wf_cdef_parent_ok) Δ.
+Proof.
+  rewrite map_Forall_lookup => c0 d0.
+  rewrite lookup_insert_Some.
+  case => [[? <-]|[?]].
+  { by rewrite /wf_cdef_parent_ok . }
+  rewrite lookup_insert_Some.
+  case => [[? <-]|[?]].
+  { by rewrite /wf_cdef_parent_ok. }
+  rewrite lookup_insert_Some.
+  case => [[? <-]|[?]].
+  { rewrite /wf_cdef_parent_ok /=.
+    econstructor => //.
+    rewrite /σ => i ty.
+    rewrite list_lookup_singleton_Some => [[? <-]].
+    by constructor.
+  }
+  rewrite lookup_singleton_Some.
+  case => [? <-].
+  by rewrite /wf_cdef_parent_ok.
+Qed.
+
+Lemma wf_constraints_ok : map_Forall (λ _cname, wf_cdef_constraints_ok) Δ.
+Proof.
+  rewrite map_Forall_lookup => c0 d0.
+  rewrite lookup_insert_Some.
+  case => [[? <-]|[?]].
+  { rewrite /wf_cdef_constraints_ok /ROBox /= /ok_constraints Forall_singleton.
+    split => /=; by repeat constructor.
+  }
+  rewrite lookup_insert_Some.
+  case => [[? <-]|[?]].
+  { rewrite /wf_cdef_constraints_ok; by constructor. }
+  rewrite lookup_insert_Some.
+  case => [[? <-]|[?]].
+  { rewrite /wf_cdef_constraints_ok; by constructor. }
+  rewrite lookup_singleton_Some.
+  case => [? <-].
+  rewrite /wf_cdef_constraints_ok; by constructor.
+Qed.
+
+Lemma wf_methods_ok : map_Forall (λ _cname, cdef_methods_ok) Δ.
+Proof.
+  rewrite map_Forall_lookup => c0 d0.
+  rewrite lookup_insert_Some.
+  case => [[? <-]|[?]].
+  { rewrite /cdef_methods_ok /ROBox /=.
+    apply map_Forall_singleton.
+    rewrite /mdef_ok /Get /=.
+    split; last by constructor.
+    by apply map_Forall_empty.
+  }
+  rewrite lookup_insert_Some.
+  case => [[? <-]|[?]].
+  { rewrite /cdef_methods_ok /Box /=.
+    rewrite map_Forall_lookup => x mx.
+    rewrite lookup_insert_Some.
+    case => [[? <-]|[?]].
+    * rewrite /mdef_ok /BoxSet /=.
+      split; last by constructor.
+      apply map_Forall_singleton.
+      by constructor.
+    * rewrite lookup_insert_Some.
+      case => [[? <-]|[?]]; last by rewrite lookup_empty.
+      rewrite /mdef_ok /Get /=.
+      split; first by apply map_Forall_empty.
+      by constructor.
+  }
+  rewrite lookup_insert_Some.
+  case => [[? <-]|[?]].
+  { rewrite /cdef_methods_ok /IntBoxS /=.
+    apply map_Forall_singleton.
+    rewrite /mdef_ok /IntBoxSSet /=.
+    split; last by constructor.
+    apply map_Forall_singleton.
+    by constructor.
+  }
+  rewrite lookup_insert_Some.
+  case => [[? <-]|[?]]; last by rewrite lookup_empty.
+  rewrite /cdef_methods_ok /Main /=.
+  apply map_Forall_singleton.
+  split; last by constructor.
+  by apply map_Forall_empty.
+Qed.
+
 Lemma wf: wf_cdefs Δ.
 Proof.
   split.
   by apply wf_extends_wf.
   by apply wf_parent.
+  by apply wf_parent_ok.
+  by apply wf_constraints_wf.
+  by apply wf_constraints_ok.
+  by apply wf_constraints_bounded.
   by apply wf_override.
   by apply wf_fields.
   by apply wf_fields_bounded.
@@ -1061,6 +1204,7 @@ Proof.
   by apply wf_methods_bounded.
   by apply wf_methods_wf.
   by apply wf_methods_mono.
+  by apply wf_methods_ok.
   by apply wf_mdefs.
   by apply wf_mono.
 Qed.
@@ -1070,7 +1214,7 @@ Qed.
  *)
 Theorem int_adequacy cmd st lty n:
   cmd_eval (main_le, main_heap "Main") cmd st n →
-  cmd_has_ty (main_lty "Main") cmd lty →
+  cmd_has_ty [] (main_lty "Main") cmd lty →
   ∀ v, lty.(ctxt) !! v = Some IntT →
   ∃ z, st.1.(lenv) !! v = Some (IntV z).
 Proof.
@@ -1085,7 +1229,11 @@ Proof.
   apply (@step_updN_soundness sem_heapΣ n).
   iMod sem_heap_init as (Hheap) "Hmain" => //.
   iModIntro.
-  iDestruct ((cmd_adequacy interp_env_empty _ _ _ wf wfinit ht _ _ _ he) with "Hmain") as "H" => /=.
+  assert (Σcoherency : Σinterp [] []) by done.
+  assert (wfΣc : Forall wf_constraint []).
+  { rewrite Forall_forall => ?. by set_solver. }
+  assert (wfΣi : interp_env_as_mixed [] []) by done.
+  iDestruct ((cmd_adequacy [] [] _ _ _ wf wfinit wfΣc wfΣi Σcoherency ht _ _ _ he) with "Hmain") as "H" => /=.
   iRevert "H".
   iApply updN_mono.
   iIntros "[Hh [Hthis Hl]]".
@@ -1098,7 +1246,7 @@ Qed.
 
 Theorem class_adequacy cmd st lty n:
   cmd_eval (main_le, main_heap "Main") cmd st n →
-  cmd_has_ty (main_lty "Main") cmd lty →
+  cmd_has_ty [] (main_lty "Main") cmd lty →
   ∀ v T σ, lty.(ctxt) !! v = Some (ClassT T σ) →
   ∃ l Tdyn vs, st.1.(lenv) !! v = Some (LocV l) ∧
           st.2 !! l = Some (Tdyn, vs) ∧
@@ -1115,7 +1263,11 @@ Proof.
   apply (@step_updN_soundness sem_heapΣ n).
   iMod sem_heap_init as (Hheap) "Hmain" => //.
   iModIntro.
-  iDestruct ((cmd_adequacy interp_env_empty _ _ _ wf wfinit ht _ _ _ he) with "Hmain") as "H" => /=.
+  assert (Σcoherency : Σinterp [] []) by done.
+  assert (wfΣc : Forall wf_constraint []).
+  { rewrite Forall_forall => ?. by set_solver. }
+  assert (wfΣi : interp_env_as_mixed [] []) by done.
+  iDestruct ((cmd_adequacy [] [] _ _ _ wf wfinit wfΣc wfΣi Σcoherency ht _ _ _ he) with "Hmain") as "H" => /=.
   iRevert "H".
   iApply updN_mono.
   iIntros "[Hh [_ Hl]]".
