theories/typing.v
@@ -14,9 +14,281 @@ Section Typing.
   Context `{PDC: ProgDefContext}.
 
   (* Helping the inference with this notation that hides Δ *)
-  Local Notation "s <: t" := (@subtype _ s t) (at level 70, no associativity).
-  Local Notation "lty <:< rty" := (@lty_sub _ lty rty) (at level 70, no associativity).
-  Local Notation "lts <: vs :> rts" := (@subtype_targs _ vs lts rts) (at level 70, vs at next level).
+  Local Notation "Γ ⊢ s <: t" := (@subtype _ Γ s t) (at level 70, s at next level, no associativity).
+  Local Notation "Γ ⊢ lty <:< rty" := (@lty_sub _ Γ lty rty) (lty at next level, at level 70, no associativity).
+
+  (* At class + substitution is `ok` w.r.t. to a set of constraints `Γ` if
+   * - all the types in the substitution are ok
+   * - all the constraints of that class are satisfied.
+   *)
+  Inductive ok_ty (Γ: list constraint) : lang_ty → Prop :=
+    | OkInt: ok_ty Γ IntT
+    | OkBool: ok_ty Γ BoolT
+    | OkNothing: ok_ty Γ NothingT
+    | OkMixed: ok_ty Γ MixedT
+    | OkClass t σ def:
+        (∀ i ty, σ !! i = Some ty → ok_ty Γ ty) →
+        Δ !! t = Some def →
+        (∀ i c, def.(constraints) !! i = Some c → Γ ⊢ (subst_ty σ c.1) <: (subst_ty σ c.2)) →
+        ok_ty Γ (ClassT t σ)
+    | OkNull: ok_ty Γ NullT
+    | OkNonNull: ok_ty Γ NonNullT
+    | OkUnion s t: ok_ty Γ s → ok_ty Γ t → ok_ty Γ (UnionT s t)
+    | OkInter s t: ok_ty Γ s → ok_ty Γ t → ok_ty Γ (InterT s t)
+    | OkGen n: ok_ty Γ (GenT n)
+    | OkEx t: ok_ty Γ (ExT t)
+  .
+
+  Lemma ok_ty_constraint_elim_ G T:
+    ok_ty G T →
+    ∀ Γ Γ', G = Γ ++ Γ' →
+    (∀ i c, Γ' !! i = Some c → Γ ⊢ c.1 <: c.2) →
+    ok_ty Γ T.
+  Proof.
+    induction 1 as [ | | | | t σ def hσ hi hdef hconstr
+    | | | s t hs hi ht hit | s t hs hi ht hit | n | t] => Γ Γ' heq hΓ; subst; try by constructor.
+    - apply OkClass with def => //.
+      + move => i ty h; by eapply hi.
+      + move => i c h.
+        apply subtype_constraint_elim with Γ'; by eauto.
+    - constructor; by eauto.
+    - constructor; by eauto.
+  Qed.
+
+  Lemma ok_ty_constraint_elim Γ Γ' T:
+    ok_ty (Γ ++ Γ') T →
+    (∀ i c, Γ' !! i = Some c → Γ ⊢ c.1 <: c.2) →
+    ok_ty Γ T.
+  Proof. intros; by eapply ok_ty_constraint_elim_. Qed.
+
+  Lemma ok_ty_weaken Γ t: ok_ty Γ t → ∀ Γ', Γ ⊆ Γ' → ok_ty Γ' t.
+  Proof.
+    induction 1 as [ | | | | t σ def hσ hi hdef hconstr
+    | | | s t hs hi ht hit | s t hs hi ht hit | n | t] => Γ' hincl; try by constructor.
+    - apply OkClass with def => //.
+      + move => i ty h; by apply hi with i.
+      + move => i c h.
+        apply subtype_weaken with Γ; by eauto.
+    - constructor; by eauto.
+    - constructor; by eauto.
+  Qed.
+
+  Lemma ok_ty_class_inv Γ t σ: ok_ty Γ (ClassT t σ) → Forall (ok_ty Γ) σ.
+  Proof.
+    move => h; inv h.
+    apply Forall_forall => x hin.
+    apply elem_of_list_lookup_1 in hin as [i hin].
+    by eauto.
+  Qed.
+
+  Lemma ok_ty_subst Γ t:
+    map_Forall (λ _, wf_cdef_parent Δ) Δ →
+    map_Forall (λ _, wf_cdef_constraints_bounded) Δ →
+    ok_ty Γ t →
+    wf_ty t →
+    ∀ Γ' σ, Forall wf_ty σ →
+         Forall (ok_ty Γ') σ →
+         ok_ty (Γ' ++ (subst_constraints σ Γ)) (subst_ty σ t).
+  Proof.
+    move => hwp hcb.
+    induction 1 as [ | | | | t σt def hσt hi hdef hconstr
+    | | | s t hs his ht hit | s t hs his ht hit | n | t ]
+    => hwf Γ' σ hwfσ hokσ /=; try (constructor; by eauto).
+    - apply OkClass with def => //.
+      + move => i ty h.
+        apply list_lookup_fmap_inv in h as [ty' [-> h]].
+        apply wf_ty_class_inv in hwf.
+        apply hi with i => //.
+        rewrite Forall_forall in hwf.
+        apply elem_of_list_lookup_2 in h.
+        by apply hwf in h.
+      + move => i c h.
+        assert (hdef' := hdef).
+        apply hcb in hdef'.
+        rewrite /wf_cdef_constraints_bounded Forall_forall in hdef'.
+        assert (h' := h).
+        apply elem_of_list_lookup_2 in h.
+        apply hdef' in h as [].
+        apply subtype_weaken with (subst_constraints σ Γ); last by set_solver.
+        rewrite -!subst_ty_subst.
+        * apply subtype_subst => //.
+          by apply hconstr with i.
+        * inv hwf; simplify_eq.
+          by rewrite H4.
+        * inv hwf; simplify_eq.
+          by rewrite H4.
+    - inv hwf.
+      constructor; by eauto.
+    - inv hwf.
+      constructor; by eauto.
+    - destruct (σ !! n) as [ ty | ] eqn:hty; last by constructor.
+      simpl.
+      rewrite Forall_forall in hokσ.
+      apply elem_of_list_lookup_2 in hty.
+      apply ok_ty_weaken with Γ'; first by apply hokσ.
+      by set_solver.
+  Qed.
+
+  Definition ok_constraint Γ (c: constraint) :=
+    ok_ty Γ c.1 ∧ ok_ty Γ c.2.
+
+  Definition ok_constraints Γ G := Forall (ok_constraint Γ) G.
+
+  Definition wf_cdef_parent_ok cdef :=
+    match cdef.(superclass) with
+    | None => True
+    | Some (parent, σ) =>
+        ok_ty cdef.(constraints) (ClassT parent σ)
+    end
+  .
+
+  Lemma extends_using_ok A B σ:
+    map_Forall (λ _cname, wf_cdef_parent_ok) Δ →
+    extends_using A B σ →
+    ∃ adef,
+    Δ !! A = Some adef ∧
+    ok_ty adef.(constraints) (ClassT B σ).
+  Proof.
+    move => hok h.
+    destruct h as [A B adef σ hΔ hsuper].
+    exists adef; split => //.
+    apply hok in hΔ.
+    by rewrite /wf_cdef_parent_ok hsuper in hΔ.
+  Qed.
+
+  Lemma gen_targs_ok Γ n:
+    ∀ i ty, gen_targs n !! i = Some ty →
+    ok_ty Γ ty.
+  Proof.
+    move => i ty /lookup_gen_targs ->.
+    by constructor.
+  Qed.
+
+  Lemma ok_ty_trans Γ ty:
+    ok_ty Γ ty →
+    ∀ Γ',
+    (∀ i c, Γ !! i = Some c → Γ' ⊢ c.1 <: c.2) →
+    ok_ty Γ' ty.
+  Proof.
+    induction 1 as [ | | | | t σ def hσ hi hdef hconstr
+    | | | s t hs hi ht hit | s t hs hi ht hit | n | t] => Γ' hΓ; try by constructor.
+    - econstructor => //.
+      + move => k ty hk; by eauto.
+      + move => k c' hc'.
+        apply hconstr in hc'.
+        apply subtype_constraint_trans with Γ; by eauto.
+    - constructor; by eauto.
+    - constructor; by eauto.
+  Qed.
+
+  Lemma inherits_using_ok A B σ:
+    map_Forall (λ _ : string, wf_cdef_parent Δ) Δ →
+    map_Forall (λ _cname, wf_cdef_parent_ok) Δ →
+    map_Forall (λ _ : string, wf_cdef_constraints_bounded) Δ →
+    inherits_using A B σ →
+    ∃ adef,
+    Δ !! A = Some adef ∧
+    ok_ty adef.(constraints) (ClassT B σ).
+  Proof.
+    move => hp hok hcb.
+    induction 1 as [ A adef hΔ | A B σ hext | A B σ C σC hext h hi ].
+    - exists adef; split => //.
+      econstructor => //.
+      + by apply gen_targs_ok.
+      + move => i c hc.
+        rewrite !subst_ty_id.
+        * constructor.
+          apply elem_of_list_lookup.
+          exists i; by rewrite hc {1}(surjective_pairing c).
+        * apply hcb in hΔ.
+          rewrite /wf_cdef_constraints_bounded Forall_forall in hΔ.
+          apply elem_of_list_lookup_2 in hc.
+          by apply hΔ in hc as [].
+        * apply hcb in hΔ.
+          rewrite /wf_cdef_constraints_bounded Forall_forall in hΔ.
+          apply elem_of_list_lookup_2 in hc.
+          by apply hΔ in hc as [].
+    - by apply extends_using_ok in hext.
+    - destruct hi as (bdef & hB & hokB).
+      destruct hext as [A B adef σ hΔ hsuper].
+      assert (hσ: Forall wf_ty σ).
+      { apply hp in hΔ.
+        rewrite /wf_cdef_parent hsuper in hΔ.
+        by repeat destruct hΔ as [? hΔ].
+      }
+      exists adef; split => //.
+      assert (hA := hΔ).
+      apply hok in hΔ.
+      rewrite /wf_cdef_parent_ok hsuper in hΔ.
+      inv hΔ; inv hokB; simplify_eq.
+      rename def0 into cdef.
+      rename H5 into hC.
+      econstructor => //.
+      { move => i ty hi.
+        apply list_lookup_fmap_inv in hi as [ty' [-> hi]].
+        eapply ok_ty_trans.
+        + eapply ok_ty_subst => //.
+          { by eauto. }
+          { apply inherits_using_wf in h as (? & ? & ? & ? & ? & ? & hF)=> //.
+            rewrite Forall_forall in hF.
+            apply hF.
+            by apply elem_of_list_lookup_2 in hi.
+          }
+          apply hok in hA.
+          rewrite /wf_cdef_parent_ok hsuper in hA.
+          apply ok_ty_class_inv in hA.
+          exact hA.
+        + move => j c.
+          rewrite lookup_app_Some.
+          case => [hc | [? ]].
+          * apply SubConstraint.
+            apply elem_of_list_lookup_2 in hc.
+            by rewrite -surjective_pairing.
+          * rewrite /subst_constraints => hc.
+            apply list_lookup_fmap_inv in hc as [c' [-> hc]].
+            rewrite /subst_constraint /=.
+            apply hok in hA.
+            rewrite /wf_cdef_parent_ok hsuper in hA.
+            inv hA; simplify_eq.
+            by eauto.
+      }
+      move => i c hc.
+      simplify_eq.
+      rewrite -!subst_ty_subst.
+      + eapply subtype_constraint_trans.
+        * apply subtype_subst => //.
+          by eauto.
+        * move => j c'.
+          rewrite /subst_constraints => hc'.
+          apply list_lookup_fmap_inv in hc' as [c'' [-> hc']].
+          rewrite /subst_constraint /=.
+          by eauto.
+      + assert (hC' := hC).
+        apply hcb in hC.
+        rewrite /wf_cdef_constraints_bounded Forall_forall in hC.
+        apply elem_of_list_lookup_2 in hc.
+        apply hC in hc as [].
+        apply inherits_using_wf in h as (? & ? & ? & ? & ? & hL & ?)=> //.
+        simplify_eq.
+        by rewrite hL.
+      + assert (hC' := hC).
+        apply hcb in hC.
+        rewrite /wf_cdef_constraints_bounded Forall_forall in hC.
+        apply elem_of_list_lookup_2 in hc.
+        apply hC in hc as [].
+        apply inherits_using_wf in h as (? & ? & ? & ? & ? & hL & ?)=> //.
+        simplify_eq.
+        by rewrite hL.
+  Qed.
+
+  Definition wf_cdef_constraints_ok cdef :=
+    ok_constraints cdef.(constraints) cdef.(constraints).
+
+  Definition mdef_ok Γ mdef : Prop :=
+    map_Forall (λ _argname, ok_ty Γ) mdef.(methodargs) ∧ ok_ty Γ mdef.(methodrettype).
+
+  Definition cdef_methods_ok cdef :=
+    map_Forall (λ _mname, mdef_ok cdef.(constraints)) cdef.(classmethods).
 
   (* Typing Judgements *)
   Definition is_bool_op op : bool :=
@@ -26,47 +298,75 @@ Section Typing.
     end
   .
 
-  Inductive expr_has_ty (lty : local_tys) :
+  Inductive expr_has_ty Γ (lty : local_tys) :
     expr → lang_ty → Prop :=
-    | IntTy : ∀ z, expr_has_ty lty (IntE z) IntT
-    | BoolTy: ∀ b, expr_has_ty lty (BoolE b) BoolT
-    | NullTy: expr_has_ty lty NullE NullT
+    | IntTy : ∀ z, expr_has_ty Γ lty (IntE z) IntT
+    | BoolTy: ∀ b, expr_has_ty Γ lty (BoolE b) BoolT
+    | NullTy: expr_has_ty Γ lty NullE NullT
     | OpIntTy: ∀ op e1 e2,
         is_bool_op op = false →
-        expr_has_ty lty e1 IntT →
-        expr_has_ty lty e2 IntT →
-        expr_has_ty lty (OpE op e1 e2) IntT
+        expr_has_ty Γ lty e1 IntT →
+        expr_has_ty Γ lty e2 IntT →
+        expr_has_ty Γ lty (OpE op e1 e2) IntT
     | OpBoolTy: ∀ op e1 e2,
         is_bool_op op = true →
-        expr_has_ty lty e1 IntT →
-        expr_has_ty lty e2 IntT →
-        expr_has_ty lty (OpE op e1 e2) BoolT
+        expr_has_ty Γ lty e1 IntT →
+        expr_has_ty Γ lty e2 IntT →
+        expr_has_ty Γ lty (OpE op e1 e2) BoolT
     | GenTy: ∀ v ty,
         lty.(ctxt) !! v = Some ty →
-        expr_has_ty lty (VarE v) ty
-    | ThisTy : expr_has_ty lty ThisE (this_type lty)
+        expr_has_ty Γ lty (VarE v) ty
+    | ThisTy : expr_has_ty Γ lty ThisE (this_type lty)
     | ESubTy: ∀ e s t,
-        expr_has_ty lty e s →
+        expr_has_ty Γ lty e s →
         wf_ty t →
-        s <: t →
-        expr_has_ty lty e t
+        ok_ty Γ t →
+        Γ ⊢ s <: t →
+        expr_has_ty Γ lty e t
   .
 
-  Lemma expr_has_ty_subst σ lty e ty:
-    map_Forall (λ _ : string, wf_cdef_parent Δ) Δ →
-    Forall wf_ty σ →
-    expr_has_ty lty e ty →
-    expr_has_ty (subst_lty σ lty) e (subst_ty σ ty).
+  Lemma expr_has_ty_constraint_elim_ G lty e ty:
+    expr_has_ty G lty e ty →
+    ∀ Γ Γ', G = Γ ++ Γ' →
+    (∀ i c, Γ' !! i = Some c → Γ ⊢ c.1 <: c.2) →
+    expr_has_ty Γ lty e ty.
   Proof.
-    move => hp hwf.
     induction 1 as [ z | b | | op e1 e2 hop h1 hi1 h2 hi2 |
-      op e1 e2 hop h1 hi1 h2 hi2 | v ty h | | e s t h hi hsub ] => //=; try (by constructor).
+      op e1 e2 hop h1 hi1 h2 hi2 | v ty h | | e s t h hi hok hsub ] => Γ Γ' heq hΓ; subst; try (by constructor).
+    - constructor; by eauto.
+    - constructor; by eauto.
+    - econstructor.
+      + by eauto.
+      + done.
+      + by eapply ok_ty_constraint_elim.
+      + by eapply subtype_constraint_elim.
+  Qed.
+
+  Lemma expr_has_ty_constraint_elim Γ Γ' lty e ty:
+    expr_has_ty (Γ ++ Γ') lty e ty →
+    (∀ i c, Γ' !! i = Some c → Γ ⊢ c.1 <: c.2) →
+    expr_has_ty Γ lty e ty.
+  Proof. intros; by eapply expr_has_ty_constraint_elim_. Qed.
+
+  Lemma expr_has_ty_subst Γ' Γ σ lty e ty:
+    map_Forall (λ _ : string, wf_cdef_parent Δ) Δ →
+    map_Forall (λ _ : string, wf_cdef_constraints_bounded) Δ →
+    Forall wf_ty σ →
+    Forall (ok_ty Γ') σ →
+    expr_has_ty Γ lty e ty →
+    expr_has_ty (Γ' ++ (subst_constraints σ Γ)) (subst_lty σ lty) e (subst_ty σ ty).
+  Proof.
+    move => hp hb hσwf hσok.
+    induction 1 as [ z | b | | op e1 e2 hop h1 hi1 h2 hi2 |
+      op e1 e2 hop h1 hi1 h2 hi2 | v ty h | | e s t h hi hok hsub ] => //=; try (by constructor).
     - constructor.
       rewrite /subst_lty /=.
       by rewrite lookup_fmap h.
     - econstructor; first by apply hi.
       + by apply wf_ty_subst.
-      + by apply subtype_subst.
+      + by apply ok_ty_subst.
+      + apply subtype_weaken with (subst_constraints σ Γ); first by apply subtype_subst.
+        by set_solver.
   Qed.
 
   Definition wf_lty lty :=
@@ -105,9 +405,9 @@ Section Typing.
       by apply hl in hk.
   Qed.
 
-  Lemma expr_has_ty_wf lty e ty:
+  Lemma expr_has_ty_wf Γ lty e ty:
     wf_lty lty →
-    expr_has_ty lty e ty →
+    expr_has_ty Γ lty e ty →
     wf_ty ty.
   Proof.
     move => hwf.
@@ -118,80 +418,130 @@ Section Typing.
   Qed.
 
   (* continuation-based typing for commands *)
-  Inductive cmd_has_ty :
-    local_tys → cmd → local_tys → Prop :=
-    | SkipTy: ∀ lty, cmd_has_ty lty SkipC lty
+  Inductive cmd_has_ty Γ : local_tys → cmd → local_tys → Prop :=
+    | SkipTy: ∀ lty, cmd_has_ty Γ lty SkipC lty
     | SeqTy: ∀ lty1 lty2 lty3 fstc sndc,
-        cmd_has_ty lty1 fstc lty2 →
-        cmd_has_ty lty2 sndc lty3 →
-        cmd_has_ty lty1 (SeqC fstc sndc) lty3
+        cmd_has_ty Γ lty1 fstc lty2 →
+        cmd_has_ty Γ lty2 sndc lty3 →
+        cmd_has_ty Γ lty1 (SeqC fstc sndc) lty3
     | LetTy: ∀ lty lhs e ty,
-        expr_has_ty lty e ty →
-        cmd_has_ty lty (LetC lhs e) (<[lhs := ty]>lty)
+        expr_has_ty Γ lty e ty →
+        cmd_has_ty Γ lty (LetC lhs e) (<[lhs := ty]>lty)
     | IfTy: ∀ lty1 lty2 cond thn els,
-        expr_has_ty lty1 cond BoolT →
-        cmd_has_ty lty1 thn lty2 →
-        cmd_has_ty lty1 els lty2 →
-        cmd_has_ty lty1 (IfC cond thn els) lty2
+        expr_has_ty Γ lty1 cond BoolT →
+        cmd_has_ty Γ lty1 thn lty2 →
+        cmd_has_ty Γ lty1 els lty2 →
+        cmd_has_ty Γ lty1 (IfC cond thn els) lty2
     | GetPrivTy: ∀ lty lhs t σ name fty,
         type_of_this lty = (t, σ) →
         has_field name t Private fty t →
-        cmd_has_ty lty (GetC lhs ThisE name) (<[lhs := subst_ty σ fty]>lty)
+        cmd_has_ty Γ lty (GetC lhs ThisE name) (<[lhs := subst_ty σ fty]>lty)
     | GetPubTy: ∀ lty lhs recv t σ name fty orig,
-        expr_has_ty lty recv (ClassT t σ) →
+        expr_has_ty Γ lty recv (ClassT t σ) →
         has_field name t Public fty orig →
-        cmd_has_ty lty (GetC lhs recv name) (<[lhs := subst_ty σ fty]>lty)
+        cmd_has_ty Γ lty (GetC lhs recv name) (<[lhs := subst_ty σ fty]>lty)
     | SetPrivTy: ∀ lty fld rhs fty t σ,
         type_of_this lty = (t, σ) →
         has_field fld t Private fty t →
-        expr_has_ty lty rhs (subst_ty σ fty) →
-        cmd_has_ty lty (SetC ThisE fld rhs) lty
+        expr_has_ty Γ lty rhs (subst_ty σ fty) →
+        cmd_has_ty Γ lty (SetC ThisE fld rhs) lty
     | SetPubTy: ∀ lty recv fld rhs fty orig t σ,
-        expr_has_ty lty recv (ClassT t σ) →
+        expr_has_ty Γ lty recv (ClassT t σ) →
         has_field fld t Public fty orig →
-        expr_has_ty lty rhs (subst_ty σ fty) →
-        cmd_has_ty lty (SetC recv fld rhs) lty
-    | NewTy: ∀ lty lhs t targs args fields (*cdef*),
+        expr_has_ty Γ lty rhs (subst_ty σ fty) →
+        cmd_has_ty Γ lty (SetC recv fld rhs) lty
+    | NewTy: ∀ lty lhs t targs args fields,
         wf_ty (ClassT t targs) →
+        ok_ty Γ (ClassT t targs) →
         has_fields t fields →
         dom (gset string) fields = dom _ args →
         (∀ f fty arg,
         fields !! f = Some fty →
         args !! f = Some arg →
-        expr_has_ty lty arg (subst_ty targs fty.1.2)) →
-        cmd_has_ty lty (NewC lhs t args) (<[lhs := ClassT t targs]>lty)
+        expr_has_ty Γ lty arg (subst_ty targs fty.1.2)) →
+        cmd_has_ty Γ lty (NewC lhs t args) (<[lhs := ClassT t targs]>lty)
     | CallTy: ∀ lty lhs recv t targs name orig mdef args,
-        expr_has_ty lty recv (ClassT t targs) →
+        expr_has_ty Γ lty recv (ClassT t targs) →
         has_method name t orig mdef →
         dom (gset string) mdef.(methodargs) = dom _ args →
         (∀ x ty arg,
         mdef.(methodargs) !! x = Some ty →
         args !! x = Some arg →
-        expr_has_ty lty arg (subst_ty targs ty)) →
-        cmd_has_ty lty (CallC lhs recv name args) (<[lhs := subst_ty targs mdef.(methodrettype)]>lty)
+        expr_has_ty Γ lty arg (subst_ty targs ty)) →
+        cmd_has_ty Γ lty (CallC lhs recv name args) (<[lhs := subst_ty targs mdef.(methodrettype)]>lty)
     | SubTy: ∀ lty c rty rty',
-        rty' <:< rty →
-        cmd_has_ty lty c rty' →
-        cmd_has_ty lty c rty
+        Γ ⊢ rty' <:< rty →
+        cmd_has_ty Γ lty c rty' →
+        cmd_has_ty Γ lty c rty
     | CondTagTy lty rty v tv t cmd :
         lty.(ctxt) !! v = Some tv →
-        lty <:< rty →
-        cmd_has_ty (<[v:=InterT tv (ExT t)]> lty) cmd rty →
-        cmd_has_ty lty (CondTagC v t cmd) rty
+        Γ ⊢ lty <:< rty →
+        cmd_has_ty Γ (<[v:=InterT tv (ExT t)]> lty) cmd rty →
+        cmd_has_ty Γ lty (CondTagC v t cmd) rty
   .
 
-  Lemma cmd_has_ty_wf lty cmd lty' :
+  Lemma cmd_has_ty_constraint_elim_ G lty cmd rty:
+    cmd_has_ty G lty cmd rty →
+    ∀ Γ Γ', G = Γ ++ Γ' →
+    (∀ i c, Γ' !! i = Some c → Γ ⊢ c.1 <: c.2) →
+    cmd_has_ty Γ lty cmd rty.
+  Proof.
+    induction 1 as [ lty | ????? h1 hi1 h2 hi2 | ???? he |
+      ????? he h1 hi1 h2 hi2 | ?????? he hf | ???????? he hf |
+      ?????? he hf hr | ???????? he hf hr | ?????? ht hok hf hdom hargs |
+      ????????? he hm hdom hargs |
+      ???? hsub h hi | ?????? hin hr h hi ] => Γ Γ' heq hΓ; subst.
+    - by econstructor.
+    - econstructor; by eauto.
+    - econstructor => //.
+      by eapply expr_has_ty_constraint_elim.
+    - econstructor => //.
+      + by eapply expr_has_ty_constraint_elim.
+      + by eauto.
+      + by eauto.
+    - econstructor; by eauto.
+    - econstructor => //.
+      by eapply expr_has_ty_constraint_elim.
+    - econstructor => //.
+      by eapply expr_has_ty_constraint_elim.
+    - econstructor => //.
+      + by eapply expr_has_ty_constraint_elim.
+      + by eapply expr_has_ty_constraint_elim.
+    - econstructor => //.
+      + by eapply ok_ty_constraint_elim.
+      + move => ?????.
+        eapply expr_has_ty_constraint_elim; by eauto.
+    - econstructor => //.
+      + by eapply expr_has_ty_constraint_elim.
+      + move => ?????.
+        eapply expr_has_ty_constraint_elim; by eauto.
+    - econstructor => //.
+      + by eapply lty_sub_constraint_elim.
+      + by eauto.
+    - eapply CondTagTy => //.
+      + by eapply lty_sub_constraint_elim.
+      + by eauto.
+  Qed.
+
+  Lemma cmd_has_ty_constraint_elim Γ Γ' lty cmd rty:
+    cmd_has_ty (Γ ++ Γ') lty cmd rty →
+    (∀ i c, Γ' !! i = Some c → Γ ⊢ c.1 <: c.2) →
+    cmd_has_ty Γ lty cmd rty.
+  Proof. intros; by eapply cmd_has_ty_constraint_elim_. Qed.
+
+  Lemma cmd_has_ty_wf Γ lty cmd lty' :
     map_Forall (λ _ : string, wf_cdef_parent Δ) Δ →
     map_Forall (λ _ : string, wf_cdef_fields_wf) Δ →
     map_Forall (λ _ : string, wf_cdef_methods_wf) Δ →
+    Forall wf_constraint Γ →
     wf_lty lty →
-    cmd_has_ty lty cmd lty' →
+    cmd_has_ty Γ lty cmd lty' →
     wf_lty lty'.
   Proof.
-    move => hp hfields hmethods [hthis hwf].
+    move => hp hfields hmethods hΓ [hthis hwf].
     induction 1 as [ lty | ????? h1 hi1 h2 hi2 | ???? he |
       ????? he h1 hi1 h2 hi2 | ?????? he hf | ???????? he hf |
-      ?????? he hf hr | ???????? he hf hr | ?????? ht hf hdom hargs |
+      ?????? he hf hr | ???????? he hf hr | ?????? ht hok hf hdom hargs |
       ????????? he hm hdom hargs |
       ???? hsub h hi | ?????? hin hr h hi ] => //=; try (by eauto).
     - apply hi2.
@@ -243,21 +593,24 @@ Section Typing.
         by apply hwf in hk.
   Qed.
 
-  Lemma cmd_has_ty_subst σ lty cmd lty':
+  Lemma cmd_has_ty_subst Γ' Γ σ lty cmd lty':
     map_Forall (λ _ : string, wf_cdef_parent Δ) Δ →
     map_Forall (λ _ : string, wf_cdef_fields_wf) Δ →
     map_Forall (λ _ : string, wf_cdef_methods_wf) Δ →
     map_Forall (λ _ : string, wf_cdef_fields_bounded) Δ →
     map_Forall (λ _ : string, cdef_methods_bounded) Δ →
+    map_Forall (λ _ : string, wf_cdef_constraints_bounded) Δ →
+    Forall wf_constraint Γ →
     wf_lty lty →
     Forall wf_ty σ →
-    cmd_has_ty lty cmd lty' →
-    cmd_has_ty (subst_lty σ lty) cmd (subst_lty σ lty').
+    Forall (ok_ty Γ') σ →
+    cmd_has_ty Γ lty cmd lty' →
+    cmd_has_ty (Γ' ++ (subst_constraints σ Γ)) (subst_lty σ lty) cmd (subst_lty σ lty').
   Proof.
-    move => hp hfields hmethods hfb hmb hwf0 hwf1.
+    move => hp hfields hmethods hfb hmb hcb hΓ hwf0 hwf1 hwf2.
     induction 1 as [ lty | ????? h1 hi1 h2 hi2 | ???? he |
       ????? he h1 hi1 h2 hi2 | ?????? he hf | ???????? he hf |
-      ?????? he hf hr | ???????? he hf hr | ?????? hwf hf hdom hargs |
+      ?????? he hf hr | ???????? he hf hr | ?????? hwf hok hf hdom hargs |
       ????????? he hm hdom hargs |
       ???? hsub h hi | ?????? hin hr h hi ] => //=.
     - by constructor.
@@ -327,6 +680,9 @@ Section Typing.
         apply wf_ty_subst => //.
         by apply H3 in hty'.
       }
+      { change (ClassT t (subst_ty σ <$> targs)) with (subst_ty σ (ClassT t targs)).
+        by apply ok_ty_subst.
+      }
       move => f [[vis fty] orig] arg hfty ha.
       rewrite -subst_ty_subst.
       + eapply expr_has_ty_subst => //.
@@ -376,11 +732,13 @@ Section Typing.
         apply expr_has_ty_wf in he => //.
         inv he; simplify_eq.
         by rewrite H2.
-    - econstructor; first by apply lty_sub_subst.
-      by apply hi.
+    - econstructor; last by apply hi.
+      apply lty_sub_weaken with (subst_constraints σ Γ); last by set_solver.
+      by apply lty_sub_subst.
     - eapply CondTagTy.
       + by rewrite lookup_fmap hin /=.
-      + by apply lty_sub_subst.
+      + apply lty_sub_weaken with (subst_constraints σ Γ); last by set_solver.
+        by apply lty_sub_subst.
       + rewrite /subst_lty fmap_insert /= in hi.
         apply hi.
         destruct lty as [[lt lσ] lty].
@@ -396,18 +754,18 @@ Section Typing.
    * method bodies must be well-formed under a generic substitution mapping
    * Ti -> Ti.
    *)
-  Definition wf_mdef_ty tag σ σ' mdef :=
+  Definition wf_mdef_ty Γ tag σ mdef :=
     ∃ rty,
     wf_lty rty ∧
-    cmd_has_ty
-      {| type_of_this := (tag, σ); ctxt := subst_ty σ' <$> mdef.(methodargs) |}
+    cmd_has_ty Γ
+      {| type_of_this := (tag, σ); ctxt := subst_ty σ <$> mdef.(methodargs) |}
       mdef.(methodbody) rty ∧
-    expr_has_ty rty mdef.(methodret) (subst_ty σ' mdef.(methodrettype))
+    expr_has_ty Γ rty mdef.(methodret) (subst_ty σ mdef.(methodrettype))
   .
 
   Definition cdef_wf_mdef_ty cname cdef :=
     let σ := gen_targs (length cdef.(generics)) in
-    map_Forall (λ _mname mdef, wf_mdef_ty cname σ σ mdef) cdef.(classmethods)
+    map_Forall (λ _mname mdef, wf_mdef_ty cdef.(constraints) cname σ mdef) cdef.(classmethods)
   .
 
   (* Collection of all program invariant (at the source level):
@@ -419,6 +777,10 @@ Section Typing.
   Record wf_cdefs (prog: stringmap classDef) := {
     wf_extends_wf : wf_no_cycle prog;
     wf_parent : map_Forall (λ _cname, wf_cdef_parent prog) prog;
+    wf_parent_ok : map_Forall (λ _cname, wf_cdef_parent_ok) prog;
+    wf_constraints_wf : map_Forall (λ _cname, wf_cdef_constraints_wf) prog;
+    wf_constraints_ok : map_Forall (λ _cname, wf_cdef_constraints_ok) prog;
+    wf_constraints_bounded : map_Forall (λ _cname, wf_cdef_constraints_bounded) prog;
     wf_override : wf_method_override prog;
     wf_fields : map_Forall (λ _cname, wf_cdef_fields) prog;
     wf_fields_bounded : map_Forall (λ _cname, wf_cdef_fields_bounded) prog;
@@ -428,6 +790,7 @@ Section Typing.
     wf_methods_bounded : map_Forall (λ _cname, cdef_methods_bounded) prog;
     wf_methods_wf : map_Forall (λ _cname, wf_cdef_methods_wf) prog;
     wf_methods_mono : map_Forall (λ _cname, wf_cdef_methods_mono) prog;
+    wf_methods_ok : map_Forall (λ _cname, cdef_methods_ok) prog;
     wf_mdefs : map_Forall cdef_wf_mdef_ty prog;
     wf_mono : map_Forall (λ _cname, wf_cdef_mono) prog;
   }
